Picinae_fault_tolerance.v
@@ -4,11 +4,17 @@ Require Import NArith.
 Module Type FaultToleranceConfig (Arch : Architecture)
                                  (IL : PICINAE_IL).
     Import IL.
+
+    Parameter w : N.
+    Parameter w_nontrivial : 1 < 2^w.
+
     Parameter fault_counter : var.
     Parameter fault_counter_typed :
-        exists w,
-            1 < 2^w /\
-            archtyps fault_counter = Some w.
+        archtyps fault_counter = Some w.
+
+    Parameter mem : var.
+    Parameter mem_typed :
+        archtyps mem = Some (8 * 2^w).
 End FaultToleranceConfig.
 
 Module FaultTolerance (Arch : Architecture)
@@ -18,29 +24,28 @@ Module FaultTolerance (Arch : Architecture)
                       (SIL : PICINAE_STATICS IL TIL).
 Import Arch IL FTC TIL SIL.
 
-Definition inject_fault (p : program) (s : store) (a : addr) :=
+Definition inject_skip (p : program) (s : store) (a : addr) :=
   match p s a with
   | None => None
   | Some (sz,q) =>
-        match archtyps fault_counter with None => None | Some w =>
         Some (sz,
               If (BinOp OP_AND (BinOp OP_LT (Word 0x0 w) (Var fault_counter)) (Unknown 1))
                 (Move fault_counter (BinOp OP_MINUS (Var fault_counter) (Word 0x1 w)))
               q)
-        end
   end.
 
 (* Only useful for architectures with a Gallina-defined lifter
    accompanied by a well-typedness theorem, eg welltyped_rv2il *)
-Lemma inject_fault_welltyped : forall p,
+Lemma inject_skip_welltyped : forall p,
     (forall s a sz instr,
         p s a = Some (sz, instr) ->
         hastyp_stmt archtyps archtyps instr archtyps) ->
-    welltyped_prog archtyps (inject_fault p).
+    welltyped_prog archtyps (inject_skip p).
 Proof.
-    intros p WT s a. unfold inject_fault.
+    intros p WT s a. unfold inject_skip.
     destruct (p s a) eqn:E; [|exact I]. destruct p0 as (sz & instr).
-    destruct fault_counter_typed as (w & BigW & FCW). rewrite FCW.
+    pose proof fault_counter_typed. pose proof mem_typed.
+    pose proof w_nontrivial.
     exists archtyps.
     econstructor.
     change 1 with (widthof_binop OP_AND 1). constructor.
@@ -50,14 +55,73 @@ Proof.
     econstructor. right. eassumption.
         change w with (widthof_binop OP_MINUS w) at 2. constructor.
         now constructor.
-        constructor. assumption.
+        now constructor. 
         eapply typchk_stmt_mono with (c := archtyps) (c0 := archtyps)
             (q := Move fault_counter (BinOp OP_MINUS (Var fault_counter) (Word 1 w))).
-            simpl. rewrite FCW. replace (1 <? 2^w) with true. rewrite N.eqb_refl.
-            pose proof (iseq_refl w). destruct H.
+            simpl. rewrite H. replace (1 <? 2^w) with true. rewrite N.eqb_refl.
+            pose proof (iseq_refl w). destruct H2.
                 now replace (w == w) with (@left (w=w) (w<>w) x).
             symmetry. now apply N.ltb_lt.
         reflexivity.
+    eapply WT, E.
+    reflexivity.
+Qed.
+
+Definition inject_memory_corruption (p : program) (s : store) (a : addr) :=
+  match p s a with
+  | None => None
+  | Some (sz,q) =>
+        match archtyps fault_counter with None => None | Some w =>
+        Some (sz,
+              If (BinOp OP_AND (BinOp OP_LT (Word 0x0 w) (Var fault_counter)) (Unknown 1))
+                (Seq (Move fault_counter (BinOp OP_MINUS (Var fault_counter) (Word 0x1 w)))
+                 (Seq q (
+                    (Move mem (Unknown (8 * 2^w)))
+                 )))
+              q)
+        end
+  end.
+
+(* Only useful for architectures with a Gallina-defined lifter
+   accompanied by a well-typedness theorem, eg welltyped_rv2il *)
+Lemma inject_memory_corruption_welltyped : forall p,
+    (forall s a sz instr,
+        p s a = Some (sz, instr) ->
+        hastyp_stmt archtyps archtyps instr archtyps) ->
+    welltyped_prog archtyps (inject_memory_corruption p).
+Proof.
+    intros p WT s a. unfold inject_memory_corruption.
+    destruct (p s a) eqn:E; [|exact I]. destruct p0 as (sz & instr).
+    pose proof fault_counter_typed. pose proof mem_typed.
+    pose proof w_nontrivial.
+    rewrite H. exists archtyps.
+    econstructor.
+    change 1 with (widthof_binop OP_AND 1). constructor.
+        change 1 with (widthof_binop OP_LT w). constructor.
+        constructor. apply mp2_gt_0. constructor. assumption.
+        constructor.
+    econstructor. econstructor. right. eassumption.
+        change w with (widthof_binop OP_MINUS w) at 2. constructor.
+        now constructor.
+        now constructor.
+        eapply typchk_stmt_mono with (c := archtyps) (c0 := archtyps)
+            (q := Move fault_counter (BinOp OP_MINUS (Var fault_counter) (Word 1 w))).
+            simpl. rewrite H. replace (1 <? 2^w) with true. rewrite N.eqb_refl.
+            pose proof (iseq_refl w). destruct H2.
+                now replace (w == w) with (@left (w=w) (w<>w) x).
+            symmetry. now apply N.ltb_lt.
+        reflexivity.
+    econstructor.
+        eapply WT, E. econstructor.
+        right. eassumption.
+        constructor.
+        eapply typchk_stmt_mono with (c := archtyps) (c0 := archtyps)
+            (q := Move mem (Unknown (8 * 2^w))).
+            unfold typchk_stmt, typchk_exp. rewrite H0.
+            pose proof (iseq_refl (8*2^w)). destruct H2.
+                now replace ((8*2^w) == (8*2^w)) with
+                    (@left ((8*2^w)=(8*2^w)) ((8*2^w)<>(8*2^w)) x).
+                reflexivity. reflexivity. reflexivity.
     eapply WT, E.
     reflexivity.
 Qed.
