Examples/br_ccopy/br_ccopy_ft_proof.v
@@ -236,7 +236,7 @@ Section FaultTolerantInvariants.
         | _ => NoInv
         end.
 
-    Definition br_ccopy_fault : program := inject_fault br_ccopy.
+    Definition br_ccopy_fault : program := inject_skip br_ccopy.
 
     Definition ft_exits0 := make_exits 0 br_ccopy_fault ft_invs.
     Definition ft_invs0 := make_invs 0 br_ccopy_fault ft_invs.
@@ -279,7 +279,7 @@ Proof using.
 
     intros.
     eapply startof_prefix in ENTRY; try eassumption.
-    eapply preservation_exec_prog in MDL; try (eassumption || apply inject_fault_lift_riscv_welltyped).
+    eapply preservation_exec_prog in MDL; try (eassumption || apply inject_skip_lift_riscv_welltyped).
     clear - PRE MDL. rename t1 into t. rename s1 into s. rename a1 into a.
 
     destruct_inv 32 PRE.
