Examples/register_checksum/register_checksum_proof.v
@@ -1,0 +1,154 @@
+Require Import register_checksum.
+Require Import Picinae_riscv.
+Import RVFaultTolerance.
+Import RISCVNotations.
+Require Import NArith.
+Require Import List.
+Require Import Lia ZifyN ZifyBool.
+
+Import ListNotations.
+Open Scope N_scope.
+
+Section Invariants.
+    Variable    a1 a2 a3 a4 a5 a6 a7
+             s0 s1 s2 s3 s4 s5 s6 s7 s8 s9 s10 s11
+             checksum : N.
+
+    Definition postcondition : Prop :=
+        (     a1 ⊕ a2 ⊕ a3 ⊕ a4 ⊕ a5 ⊕ a6 ⊕ a7 ⊕
+         s0 ⊕ s1 ⊕ s2 ⊕ s3 ⊕ s4 ⊕ s5 ⊕ s6 ⊕ s7 ⊕ s8 ⊕ s9 ⊕ s10 ⊕ s11
+            = checksum).
+
+    Definition regs (s : store) : Prop :=
+        s R_A0 = checksum /\
+        s R_A1 = a1 /\
+        s R_A2 = a2 /\
+        s R_A3 = a3 /\
+        s R_A4 = a4 /\
+        s R_A5 = a5 /\
+        s R_A6 = a6 /\
+        s R_A7 = a7 /\
+
+        s R_S0 = s0 /\
+        s R_S1 = s1 /\
+        s R_S2 = s2 /\
+        s R_S3 = s3 /\
+        s R_S4 = s4 /\
+        s R_S5 = s5 /\
+        s R_S6 = s6 /\
+        s R_S7 = s7 /\
+        s R_S8 = s8 /\
+        s R_S9 = s9 /\
+        s R_S10 = s10 /\
+        s R_S11 = s11.
+
+    Definition invs T (Inv Post: inv_type T) (NoInv:T) (s:store) (a:addr) : T :=
+        match a with
+        | 0x0 => Inv 0 (regs s)
+        | 0x1c0 | 0x1c4 => Post 0 (~ postcondition)
+        | 0x1c8 | 0x1cc => Post 0 (postcondition)
+        | _ => NoInv
+        end.
+
+    Definition register_checksum : program :=
+        lift_riscv register_checksum.
+
+    Definition exits0 := make_exits 0 register_checksum invs.
+    Definition invs0 := make_invs 0 register_checksum invs.
+End Invariants.
+
+(* Proof in fault-free context *)
+Theorem register_checksum_correctness:
+  forall s t xs' a1 a2 a3 a4 a5 a6 a7
+                     s0 s1 s2 s3 s4 s5 s6 s7 s8 s9 s10 s11
+                     checksum
+         (ENTRY: startof t xs' = (Addr 0, s))
+         (MDL: models rvtypctx s)
+         (REGS: regs a1 a2 a3 a4 a5 a6 a7
+                     s0 s1 s2 s3 s4 s5 s6 s7 s8 s9 s10 s11
+                     checksum s),
+  satisfies_all register_checksum 
+        (invs0 a1 a2 a3 a4 a5 a6 a7
+               s0 s1 s2 s3 s4 s5 s6 s7 s8 s9 s10 s11
+               checksum)
+        (exits0 a1 a2 a3 a4 a5 a6 a7
+                s0 s1 s2 s3 s4 s5 s6 s7 s8 s9 s10 s11
+                checksum) (xs'::t).
+Proof using.
+    Local Ltac step := time r5_step.
+    intros. apply prove_invs.
+
+    simpl. rewrite ENTRY. step. now unfold regs in REGS.
+
+    intros.
+    eapply startof_prefix in ENTRY; try eassumption.
+    eapply preservation_exec_prog in MDL; try (eassumption || apply lift_riscv_welltyped).
+    clear - PRE MDL. rename t1 into t. rename s12 into s. rename a0 into a.
+
+    destruct_inv 32 PRE.
+
+    destruct PRE as
+        (CHK & A1 & A2 & A3 & A4 & A5 & A6 & A7 &
+          S0 & S1 & S2 & S3 & S4 & S5 & S6 & S7 & S8 & S9 & S10 & S11).
+
+    repeat step.
+    - lia.
+    - discriminate.
+    - intro Contra. unfold postcondition in Contra.
+      psimpl in Contra. lia.
+Qed.
+
+Section FaultTolerantInvariants.
+    Variable    a1 a2 a3 a4 a5 a6 a7
+                s0 s1 s2 s3 s4 s5 s6 s7 s8 s9 s10 s11
+                checksum : N.
+
+    Definition register_checksum_faulty : program :=
+        inject_memory_corruption (inject_skip register_checksum).
+
+    Definition invs' :=
+            invs a1 a2 a3 a4 a5 a6 a7
+                 s0 s1 s2 s3 s4 s5 s6 s7 s8 s9 s10 s11
+                 checksum.
+
+    Definition exits0' := make_exits 0 register_checksum_faulty invs'.
+    Definition invs0' := make_invs 0 register_checksum_faulty invs'.
+End FaultTolerantInvariants.
+
+(* Proof in single-fault context *)
+Theorem register_checksum_correctness_faulty:
+  forall s t xs' a1 a2 a3 a4 a5 a6 a7
+                     s0 s1 s2 s3 s4 s5 s6 s7 s8 s9 s10 s11
+                     checksum
+         (ENTRY: startof t xs' = (Addr 0, s))
+         (MDL: models rvtypctx s)
+         (REGS: regs a1 a2 a3 a4 a5 a6 a7
+                     s0 s1 s2 s3 s4 s5 s6 s7 s8 s9 s10 s11
+                     checksum s),
+  satisfies_all register_checksum 
+        (invs0' a1 a2 a3 a4 a5 a6 a7
+                s0 s1 s2 s3 s4 s5 s6 s7 s8 s9 s10 s11
+                checksum)
+        (exits0' a1 a2 a3 a4 a5 a6 a7
+                 s0 s1 s2 s3 s4 s5 s6 s7 s8 s9 s10 s11
+                 checksum) (xs'::t).
+Proof using.
+    intros. apply prove_invs.
+
+    simpl. rewrite ENTRY. step. now unfold regs in REGS.
+
+    intros.
+    eapply startof_prefix in ENTRY; try eassumption.
+    eapply preservation_exec_prog in MDL; try (eassumption || apply lift_riscv_welltyped).
+    clear - PRE MDL. rename t1 into t. rename s12 into s. rename a0 into a.
+
+    destruct_inv 32 PRE.
+
+    destruct PRE as
+        (CHK & A1 & A2 & A3 & A4 & A5 & A6 & A7 &
+          S0 & S1 & S2 & S3 & S4 & S5 & S6 & S7 & S8 & S9 & S10 & S11).
+
+    repeat step; try lia;
+        intro Contra; unfold postcondition in Contra;
+        psimpl in Contra; lia.
+Qed.
